Improve a lot of stuff

main/Extracted.in.hs
@@ -1,0 +1,79 @@
+{-# OPTIONS_GHC -cpp -XMagicHash #-}
+{-# LANGUAGE StandaloneDeriving #-}
+
+{- For Hugs, use the option -F"cpp -P -traditional" -}
+
+module Extracted where
+import qualified Prelude
+
+import qualified GHC.Base
+import qualified GHC.Prim
+import qualified Data.Bits
+import qualified Data.Char
+import qualified Debug.Trace
+
+import Prelude (Show, (.), ($), show, (++), concat)
+import Data.List (intersperse)
+
+deriving instance Show Local_id
+deriving instance Show Frame
+
+instance Show Expr_hole where
+  show Expr_hole_id = "\x00B7"
+  show (Expr_hole_seq e1 e2) = show e1 ++ "; " ++ show e2
+  show (Expr_hole_recover e) = "recover " ++ show e
+  show (Expr_hole_assign_local n e) = n ++ " = " ++ show e
+  show (Expr_hole_field e n) = show e ++ "." ++ n
+  show (Expr_hole_assign_field1 e1 n e2) = show e1 ++ "." ++ n ++ " = " ++ show e2
+  show (Expr_hole_assign_field2 e1 n t) = show e1 ++ "." ++ n ++ " = $" ++ show t
+  show (Expr_hole_call1 e0 n ts e es) = show e0 ++ "." ++ n ++ "(" ++ (concat . intersperse ", " $ (Prelude.map (\t -> "$"++show t) ts ++ [show e] ++ Prelude.map show (list_expr_uncoerce es))) ++ ")"
+  show (Expr_hole_call2 e0 n ts) = show e0 ++ "." ++ n ++ "(" ++ (concat . intersperse ", " . Prelude.map (\t -> "$"++show t) $ ts) ++ ")"
+  show (Expr_hole_ctor n m ts e es) = n ++ "." ++ m ++ "(" ++ (concat . intersperse ", " $ (Prelude.map (\t -> "$"++show t) ts ++ [show e] ++ Prelude.map show (list_expr_uncoerce es))) ++ ")"
+
+instance Show Expr where
+  show (Expr_temp t) = "$" ++ show t
+  show (Expr_null) = "null"
+  show (Expr_seq e1 e2) = show e1 ++ "; " ++ show e2
+  show (Expr_recover e) = "recover " ++ show e
+  show (Expr_local n) = n
+  show (Expr_assign_local n e) = n ++ " = " ++ show e
+  show (Expr_field e n) = show e ++ "." ++ n
+  show (Expr_assign_field e1 n e2) = show e1 ++ "." ++ n ++ " = " ++ show e2
+  show (Expr_call e1 n es) = show e1 ++ "." ++ n ++ "(" ++ (concat . intersperse ", " . Prelude.map show . list_expr_uncoerce $ es) ++ ")"
+  show (Expr_ctor n m es) = n ++ "." ++ m ++ "(" ++ (concat . intersperse ", " . Prelude.map show . list_expr_uncoerce $ es) ++ ")"
+  
+instance Show Value where
+  show V_null = "null"
+  show (V_addr addr) = "#" ++ show (Extracted.n_to_nat addr)
+
+instance Show Extracted.Cap where
+  show Extracted.Cap_iso = "iso"
+  show Extracted.Cap_tag = "tag"
+  show Extracted.Cap_ref = "ref"
+
+instance Show Extracted.Ecap where
+  show Extracted.Cap_iso_eph = "iso^"
+  show (Extracted.Ecap_cap c) = show c
+
+instance Show Extracted.Ty where
+  show (Extracted.Ty_name name cap) = name ++ " " ++ show cap
+
+instance Show Extracted.Object where
+  show (Extracted.Build_object name fields) =
+    name ++ " { " ++ concat (intersperse ", " (Prelude.map (\(k,v) -> k ++ ": " ++ show v ) (Extracted.fields_to_list fields))) ++ " }"
+
+instance Show Extracted.N where
+  show = show . Extracted.n_to_nat
+
+instance Show Extracted.Positive where
+  show = show . Extracted.p_to_nat
+
+instance (Show a) => Show (Stringmap a) where
+  show = show . Extracted.map_to_list Extracted.stringmap_to_list 
+
+instance (Show a) => Show (Nmap a) where
+  show = show . Extracted.map_to_list Extracted.nto_list 
+
+instance (Show a) => Show (Pmap a) where
+  show = show . Extracted.map_to_list Extracted.pto_list 
+
