main/Main.hs
@@ -1,5 +1,3 @@
-{-# LANGUAGE StandaloneDeriving #-}
-
 import Control.Monad.State.Lazy
 import Control.Monad.Except
 import Data.Char
@@ -8,71 +6,12 @@ import System.IO
 import Text.Parsec (parse)
 import Text.Parsec.Combinator (eof)
 import System.Environment (getArgs)
+import qualified Text.ParserCombinators.Parsec as Parsec
 
 import qualified Parser
-import Extracted (Program, Expr(..), Expr_hole(..), Heap, Value(..), Local_id(..), Frame, Ty, Ty_ctx)
+import Extracted (Program, Expr(..), Expr_hole(..), Heap, Value(..), Local_id(..), Frame, Ty(..), Cap(..), Ty_ctx)
 import Extracted (Nmap, Pmap, Stringmap, list_expr_uncoerce)
 import qualified Extracted
-
-deriving instance Show Local_id
-deriving instance Show Extracted.Def
-deriving instance Show Extracted.Item
-deriving instance Show Extracted.Item_stub
-deriving instance Show Frame
-
-instance Show Expr_hole where
-  show Expr_hole_id = "\x00B7"
-  show (Expr_hole_seq e1 e2) = show e1 ++ "; " ++ show e2
-  show (Expr_hole_recover e) = "recover " ++ show e
-  show (Expr_hole_assign_local n e) = n ++ " = " ++ show e
-  show (Expr_hole_field e n) = show e ++ "." ++ n
-  show (Expr_hole_assign_field1 e1 n e2) = show e1 ++ "." ++ n ++ " = " ++ show e2
-  show (Expr_hole_assign_field2 e1 n t) = show e1 ++ "." ++ n ++ " = " ++ show t
-  show (Expr_hole_call1 e0 n ts e es) = show e0 ++ "." ++ n ++ "(" ++ (concat . intersperse ", " $ (map show ts ++ [show e] ++ map show (list_expr_uncoerce es))) ++ ")"
-  show (Expr_hole_call2 e0 n ts) = show e0 ++ "." ++ n ++ "(" ++ (concat . intersperse ", " . map show $ ts) ++ ")"
-  show (Expr_hole_ctor n m ts e es) = n ++ "." ++ m ++ "(" ++ (concat . intersperse ", " $ (map show ts ++ [show e] ++ map show (list_expr_uncoerce es))) ++ ")"
-
-instance Show Expr where
-  show (Expr_temp t) = show t
-  show (Expr_seq e1 e2) = show e1 ++ "; " ++ show e2
-  show (Expr_recover e) = "recover " ++ show e
-  show (Expr_local n) = n
-  show (Expr_assign_local n e) = n ++ " = " ++ show e
-  show (Expr_field e n) = show e ++ "." ++ n
-  show (Expr_assign_field e1 n e2) = show e1 ++ "." ++ n ++ " = " ++ show e2
-  show (Expr_call e1 n es) = show e1 ++ "." ++ n ++ "(" ++ (concat . intersperse ", " . map show . list_expr_uncoerce $ es) ++ ")"
-  show (Expr_ctor n m es) = n ++ "." ++ m ++ "(" ++ (concat . intersperse ", " . map show . list_expr_uncoerce $ es) ++ ")"
-  
-instance Show Value where
-  show V_null = "null"
-  show (V_addr addr) = "#" ++ show (Extracted.n_to_nat addr)
-
-instance Show Extracted.Cap where
-  show Extracted.Cap_iso = "iso"
-  show Extracted.Cap_tag = "tag"
-  show Extracted.Cap_ref = "ref"
-
-instance Show Extracted.Ty where
-  show (Extracted.Ty_name name cap) = name ++ " " ++ show cap
-
-instance Show Extracted.Object where
-  show (Extracted.Build_object name fields) =
-    name ++ " { " ++ concat (intersperse ", " (map (\(k,v) -> k ++ ": " ++ show v ) (Extracted.fields_to_list fields))) ++ " }"
-
-instance Show Extracted.N where
-  show = show . Extracted.n_to_nat
-
-instance Show Extracted.Positive where
-  show = show . Extracted.p_to_nat
-
-instance (Show a) => Show (Stringmap a) where
-  show = show . Extracted.map_to_list Extracted.stringmap_to_list 
-
-instance (Show a) => Show (Nmap a) where
-  show = show . Extracted.map_to_list Extracted.nto_list 
-
-instance (Show a) => Show (Pmap a) where
-  show = show . Extracted.map_to_list Extracted.pto_list 
 
 data ST = ST { stProg :: Program, stHeap :: Heap, stStack :: [Frame], stCtx :: Ty_ctx }
 type Repl = StateT ST (ExceptT String IO)
@@ -95,6 +34,7 @@ multiline = liftIO (multiline' [])
 load :: String -> Repl ()
 load contents = do
   prog <- parser Parser.prog contents
+  liftIO (print (Extracted.wf_program prog))
   liftIO (print prog)
   put (ST prog init_heap init_stack init_tyctx)
 
@@ -107,29 +47,41 @@ parser p line =
     Right e -> return e
     Left err -> throwError (show err)
 
+ck_expr :: Expr -> Repl Ty
+ck_expr expr = do
+  (ST prog _ _ ctx) <- get
+
+  case Extracted.ck_expr prog ctx expr of
+    Just ty -> return ty
+    Nothing -> throwError "typecheck error"
+
 evaluate' :: Expr -> Repl Value
 evaluate' expr = do
   (ST prog heap stack ctx) <- get
-  -- liftIO . putStr . unlines  $ map (("- "++) . show) stack ++ ["  " ++ show expr]
+  liftIO . putStrLn $ show (length stack - 1) ++ ": " ++ show expr
 
   case (expr, stack) of
     (Expr_temp temp, [frame]) ->
       let Just x = Extracted.lookup (Extracted.frame_lookup Extracted.localmap_lookup_temp) temp frame in return x
+
     _ -> case Extracted.eval prog heap stack expr of
       Just ((heap', stack'), expr') -> put (ST prog heap' stack' ctx) >> evaluate' expr'
       Nothing -> throwError "eval error"
 
 evaluate :: Expr -> Repl (Ty, Value)
 evaluate expr = do
-  (ST prog _ _ ctx) <- get
-  case Extracted.ck_expr prog ctx expr of
-    Just ty -> (,) ty <$> evaluate' expr
-    Nothing -> throwError "typecheck error"
+  ty <- ck_expr expr
+  val <- evaluate' expr
+  return (ty, val)
 
 command :: String -> String -> Repl ()
-command "heap"  _ = do
+command "heap" _ = do
   heap <- Extracted.heap_to_list <$> gets stHeap
   liftIO (mapM_ (\(x, o) -> putStrLn ("#" ++ show x ++ ": " ++ show o)) heap)
+
+command "stack" _ = do
+  stack <- gets stStack
+  liftIO . print $ stack
 
 command "ctx" _ = do
   ctx <- gets stCtx
@@ -150,8 +102,22 @@ repl (':':line) =
   command c (dropWhile isSpace rest)
 
 repl ('l':'e':'t':' ':line) = do
-  (x, ty) <- parser ((,) <$> Parser.identifier <* Parser.colon <*> Parser.ty) line
+  (x, ty, expr) <- parser parseLet line
+  ty <- case (ty, expr) of
+    (Just ty, _) -> return ty
+    (Nothing, Just expr) -> ck_expr expr
+
   modify (\s -> s { stCtx = tyctx_insert x ty (stCtx s) })
+  case expr of
+    Just expr -> evaluate (Expr_assign_local x expr) >> return ()
+    Nothing -> return ()
+
+  where
+    parseLet = do
+      x <- Parser.identifier
+      ty <- Parsec.optionMaybe (Parser.colon >> Parser.ty)
+      expr <- Parsec.optionMaybe (Parser.reservedOp "=" >> Parser.expr)
+      return (x, ty, expr)
 
 repl line = do
   e <- parser Parser.expr line
@@ -170,7 +136,7 @@ repl line = do
 main :: IO ()
 main = do
   args <- getArgs
-  result <- runExceptT . flip evalStateT (ST [] init_heap init_stack init_tyctx) $ do
+  result <- runExceptT . flip evalStateT (ST ((([],[]),[]),[]) init_heap init_stack init_tyctx) $ do
     prog <- case args of
       [] -> return ()
       (path : _) -> loadFile path
