src/Semantics.v
@@ -1,4 +1,3 @@
-(*
 Require Import ch2o.prelude.base.
 Require Import ch2o.prelude.option.
 Require Import Coq.Lists.List.
@@ -9,230 +8,116 @@ Require Import Ast.
 Require Import Store.
 Require Import Entities.
 
-Reserved Notation "LHS '⇒' RHS" (at level 40).
-
 Open Scope string_scope.
 
+Section step.
+Context (p: program).
+
 Inductive step : heap * list frame * expr -> heap * list frame * expr -> Prop :=
-| E_Seq : forall χ φ t e stack,
-    (χ, φ :: stack, expr_seq (expr_temp t) e) ⇒ (χ, φ :: stack, e)
+| step_hole : forall χ χ' φ φ' σ e e' ectx,
+    step (χ, φ::σ, e) (χ, φ'::σ, e') ->
+    step (χ, φ::σ, fill_hole ectx e) (χ', φ'::σ, fill_hole ectx e')
 
-| E_Recover : forall χ φ t stack,
-    (χ, φ :: stack, expr_recover (expr_temp t)) ⇒ (χ, φ :: stack, (expr_temp t))
+| step_seq : forall χ σ t e,
+    step (χ, σ, expr_seq (expr_temp t) e)
+         (χ, σ, e)
 
-| E_Local : forall χ φ t φ' x stack,
-    not (elem_of t φ) ->
+| step_recover : forall χ σ t,
+    step (χ, σ, expr_recover (expr_temp t))
+         (χ, σ, (expr_temp t))
+
+| step_local : forall χ φ σ t φ' x,
+    not (t ∈ φ) ->
     φ' = <[t := φ !!! x]> φ ->
-    (χ, φ :: stack, expr_local x) ⇒ (χ, φ' :: stack, expr_temp t)
+    step (χ, φ::σ, expr_local x)
+         (χ, φ'::σ, expr_temp t)
 
-| E_Asn_Local : forall χ φ φ' t t' x stack,
-    not (elem_of t' φ) ->
+| step_asn_local : forall χ φ φ' σ t t' x,
+    not (t' ∈ φ) ->
     φ' = <[t' := φ !!! x]>(<[x := φ !!! t]>φ) ->
-    (χ, φ :: stack, expr_assign_local x (expr_temp t)) ⇒ (χ, φ' :: stack, expr_temp t')
+    step (χ, φ::σ, expr_assign_local x (expr_temp t))
+         (χ, φ'::σ, expr_temp t')
 
-| E_Fld : forall χ φ φ' t t' f addr stack,
-    not (elem_of t' φ) ->
-    v_addr addr = φ !!! t ->
-    φ' = <[t' := χ !!! (addr, f)]> φ ->
-    (χ, φ :: stack, expr_field (expr_temp t) f) ⇒ (χ, φ' :: stack, expr_temp t')
+| step_field : forall χ φ φ' σ t t' f ω,
+    not (t' ∈ φ) ->
+    v_addr ω = φ !!! t ->
+    φ' = <[t' := χ !!! (ω, f)]> φ ->
+    step (χ, φ::σ, expr_field (expr_temp t) f)
+         (χ, φ'::σ, expr_temp t')
 
-| E_Asn_Fld : forall χ χ' φ φ' t t' t'' f addr stack,
-    not (elem_of t'' φ) ->
-    v_addr addr = φ !!! t ->
-    φ' = <[t'' := χ !!! (addr, f)]>φ ->
-    χ' = <[(addr, f) := φ !!! t']>χ ->
+| step_asn_field : forall χ χ' φ φ' σ t t' t'' f ω,
+    not (t'' ∈ φ) ->
+    v_addr ω = φ !!! t ->
+    φ' = <[t'' := χ !!! (ω, f)]>φ ->
+    χ' = <[(ω, f) := φ !!! t']>χ ->
 
-    (χ, φ :: stack, expr_assign_field (expr_temp t) f(expr_temp t')) ⇒
-    (χ', φ' :: stack, expr_temp t'')
+    step (χ, φ::σ, expr_assign_field (expr_temp t) f (expr_temp t'))
+           (χ', φ'::σ, expr_temp t'')
 
-| E_Sync : forall χ φ φ' φ'' t hole e0 name stack addr,
-    v_addr addr = φ !!! t ->
+| step_sync : forall χ φ φ' φ'' σ ectx t m e ts ω,
+    v_addr ω = φ !!! t ->
 
     φ'' = {|
-      method := name;
-      locals := <["this" := (v_addr addr)]>empty;
+      method := m;
+      locals := <["this" := (v_addr ω)]>empty;
       hole := expr_hole_id
     |} ->
 
     φ' = {|
       method := φ.(method);
       locals := φ.(locals);
-      hole := hole
+      hole := ectx
     |} ->
-    
-    make_hole e0 (expr_call (expr_temp t) name nil) hole ->
 
-    (χ, φ :: stack, e0) ⇒ (χ, φ'' :: φ' :: stack, (expr_local "this"))
+    step (χ, φ :: σ, fill_hole ectx (expr_call (expr_temp t) m (list_expr_temps ts)))
+         (χ, φ'' :: φ' :: σ, e)
 
-| E_Return : forall χ φ φ' φ'' hole t t' stack,
-    not (elem_of t' φ) ->
+| step_ctor : forall χ χ' ω φ φ' φ'' σ ectx kt k e ts,
+    not (ω ∈ heap_dom χ) ->
+    χ' = <[ω := {| name := kt; fields := empty |}]>χ ->
 
     φ'' = {|
-      method := φ.(method);
-      locals := <[t' := φ' !!! t]>φ.(locals);
+      method := k;
+      locals := <["this" := (v_addr ω)]>empty;
       hole := expr_hole_id
     |} ->
 
-    (χ, φ' :: φ :: stack, expr_temp t) ⇒
-    (χ, φ'' :: stack, fill_hole φ.(hole) (expr_temp t'))
+    φ' = {|
+      method := φ.(method);
+      locals := φ.(locals);
+      hole := ectx
+    |} ->
 
-| E_Fld_Null : forall χ φ t f stack,
-    φ !!! t = v_null ->
+    step (χ, φ :: σ, fill_hole ectx (expr_ctor kt k (list_expr_temps ts)))
+         (χ', φ'' :: φ' :: σ, e)
 
-    (χ, φ :: stack, expr_field (expr_temp t) f) ⇒
-    (χ, φ :: stack, expr_temp t)
+| step_return : forall χ φ φ' φ'' t t' σ,
+    not (t' ∈ φ) ->
+    φ'' = {|
+        method := φ.(method);
+        locals := <[t' := φ' !!! t]>φ.(locals);
+        hole := φ.(hole);
+    |} ->
+    step (χ, φ' :: φ :: σ, expr_temp t)
+         (χ, φ'' :: σ, fill_hole φ.(hole) (expr_temp t'))
 
-| E_Asn_Fld_Null : forall χ φ t t' f stack,
-    φ !!! t = v_null ->
+| step_field_null : forall χ φ σ t f,
+    v_null = φ !!! t ->
 
-    (χ, φ :: stack, expr_assign_field (expr_temp t) f (expr_temp t')) ⇒
-    (χ, φ :: stack, expr_temp t)
+    step (χ, φ::σ, expr_field (expr_temp t) f)
+         (χ, φ::σ, expr_temp t)
 
-| E_Call_Null : forall χ φ t name stack,
-    φ !!! t = v_null ->
+| step_asn_field_null : forall χ φ σ t t' f,
+    v_null = φ !!! t ->
 
-    (χ, φ :: stack, expr_call (expr_temp t) name nil) ⇒
-    (χ, φ :: stack, expr_temp t)
+    step (χ, φ::σ, expr_assign_field (expr_temp t) f (expr_temp t'))
+         (χ, φ::σ, expr_temp t)
 
-| E_Seq1 : forall χ χ' φ φ' e1 e1' e2 stack,
-    (χ, φ :: stack, e1) ⇒ (χ', φ' :: stack, e1') ->
-    (χ, φ :: stack, expr_seq e1 e2) ⇒ (χ', φ' :: stack, expr_seq e1' e2)
+| step_call_null : forall χ φ σ t n ts,
+    v_null = φ !!! t ->
 
-| E_Recover1 : forall χ χ' φ φ' e e' stack,
-    (χ, φ :: stack, e) ⇒ (χ', φ' :: stack, e') ->
-    (χ, φ :: stack, expr_recover e) ⇒ (χ', φ' :: stack, expr_recover e')
+    step (χ, φ::σ, expr_call (expr_temp t) n (list_expr_temps ts))
+         (χ, φ::σ, expr_temp t)
+.
 
-| E_Asn_Local1 : forall χ χ' φ φ' name e e' stack,
-    (χ, φ :: stack, e) ⇒ (χ', φ' :: stack, e') ->
-    (χ, φ :: stack, expr_assign_local name e) ⇒ (χ', φ' :: stack, expr_assign_local name e')
-
-| E_Fld1 : forall χ χ' φ φ' e e' name stack,
-    (χ, φ :: stack, e) ⇒ (χ', φ' :: stack, e') ->
-    (χ, φ :: stack, expr_field e name) ⇒ (χ', φ' :: stack, expr_field e' name)
-
-| E_Asn_Fld1 : forall χ χ' φ φ' e1 e1' e2 name stack,
-    (χ, φ :: stack, e1) ⇒ (χ', φ' :: stack, e1') ->
-
-    (χ, φ :: stack, expr_assign_field e1 name e2) ⇒
-    (χ', φ' :: stack, expr_assign_field e1' name e2)
-
-| E_Asn_Fld2 : forall χ χ' φ φ' t1 e2 e2' name stack,
-    (χ, φ :: stack, e2) ⇒ (χ', φ' :: stack, e2') ->
-
-    (χ, φ :: stack, expr_assign_field (expr_temp t1) name e2) ⇒
-    (χ', φ' :: stack, expr_assign_field (expr_temp t1) name e2')
-
-where "LHS '⇒' RHS" := (step LHS RHS).
-
-Reserved Notation "LHS '⇒*' RHS" (at level 40).
-
-Inductive multistep : heap * list frame * expr -> heap * list frame * expr -> Prop :=
-| multi_refl : forall h f e, (h, f, e) ⇒* (h, f, e)
-
-| multi_trans : forall h1 f1 e1 h2 f2 e2 h3 f3 e3 stack,
-    (h1, f1::stack, e1) ⇒ (h2, f2::stack, e2) ->
-    (h2, f2::stack, e2) ⇒* (h3, f3::stack, e3) ->
-    (h1, f1::stack, e1) ⇒* (h3, f3::stack, e3)
-where "LHS '⇒*' RHS" := (multistep LHS RHS).
-
-Theorem multi_one : forall h1 f1 e1 h2 f2 e2 stack,
-  (h1, f1 :: stack, e1) ⇒ (h2, f2 :: stack, e2) ->
-  (h1, f1 :: stack, e1) ⇒* (h2, f2 :: stack, e2).
-Proof.
-intros.
-apply multi_trans with (h2 := h2) (f2 := f2) (e2 := e2).
-exact H.
-apply multi_refl.
-Qed.
-
-Theorem multi_concat : forall h1 f1 e1 h2 f2 e2 h3 f3 e3 stack,
-  (h1, f1 :: stack, e1) ⇒* (h2, f2 :: stack, e2) ->
-  (h2, f2 :: stack, e2) ⇒* (h3, f3 :: stack, e3) ->
-  (h1, f1 :: stack, e1) ⇒* (h3, f3 :: stack, e3).
-Proof.
-intros.
-generalize dependent h3.
-generalize dependent f3.
-generalize dependent e3.
-dependent induction H.
-- intros. exact H0.
-- intros. apply multi_trans with h4 f4 e4.
-  exact H. apply IHmultistep. exact H1.
-Qed.
-
-Lemma E_RecoverN : forall h h' f f' e e' stack,
-    (h, f :: stack, e) ⇒* (h', f' :: stack, e') ->
-    (h, f :: stack, expr_recover e) ⇒* (h', f' :: stack, expr_recover e').
-Proof.
-intros.
-dependent induction H.
-- apply multi_refl.
-- apply multi_trans with (h2 := h2) (f2 := f2) (e2 := expr_recover e2).
-  apply E_Recover1. exact H.
-  apply IHmultistep.
-Qed.
-
-Lemma E_SeqN : forall h h' f f' e1 e1' e2 stack,
-    (h, f :: stack, e1) ⇒* (h', f' :: stack, e1') ->
-    (h, f :: stack, expr_seq e1 e2) ⇒* (h', f' :: stack, expr_seq e1' e2).
-Proof.
-intros.
-dependent induction H.
-- apply multi_refl.
-- apply multi_trans with (h2 := h2) (f2 := f2) (e2 := expr_seq e0 e2).
-  apply E_Seq1. exact H.
-  apply IHmultistep.
-Qed.
-
-Lemma E_Asn_LocalN : forall h h' f f' name e e' stack,
-    (h, f :: stack, e) ⇒* (h', f' :: stack, e') ->
-    (h, f :: stack, expr_assign_local name e) ⇒* (h', f' :: stack, expr_assign_local name e').
-Proof.
-intros.
-dependent induction H.
-- apply multi_refl.
-- apply multi_trans with (h2 := h2) (f2 := f2) (e2 := expr_assign_local name e2).
-  apply E_Asn_Local1. exact H.
-  apply IHmultistep.
-Qed.
-
-Lemma E_FldN : forall h h' f f' e e' name stack,
-    (h, f :: stack, e) ⇒* (h', f' :: stack, e') ->
-    (h, f :: stack, expr_field e name) ⇒* (h', f' :: stack, expr_field e' name).
-Proof.
-intros.
-dependent induction H.
-- apply multi_refl.
-- apply multi_trans with (h2 := h2) (f2 := f2) (e2 := expr_field e2 name).
-  apply E_Fld1. exact H.
-  apply IHmultistep.
-Qed.
-
-Lemma E_Asn_Fld1N : forall h h' f f' e1 e1' e2 name stack,
-    (h, f :: stack, e1) ⇒* (h', f' :: stack, e1') ->
-
-    (h, f :: stack, expr_assign_field e1 name e2) ⇒*
-    (h', f' :: stack, expr_assign_field e1' name e2).
-Proof.
-intros.
-dependent induction H.
-apply multi_refl.
-- apply multi_trans with (h2 := h2) (f2 := f2) (e2 := expr_assign_field e0 name e2).
-  apply E_Asn_Fld1. exact H.
-  apply IHmultistep.
-Qed.
-
-Lemma E_Asn_Fld2N : forall h h' f f' t1 e2 e2' name stack,
-    (h, f :: stack, e2) ⇒* (h', f' :: stack, e2') ->
-
-    (h, f :: stack, expr_assign_field (expr_temp t1) name e2) ⇒*
-    (h', f' :: stack, expr_assign_field (expr_temp t1) name e2').
-Proof.
-intros.
-dependent induction H.
-apply multi_refl.
-- apply multi_trans with (h2 := h2) (f2 := f2) (e2 := expr_assign_field (expr_temp t1) name e0).
-  apply E_Asn_Fld2. exact H.
-  apply IHmultistep.
-Qed.
-*)
+End step.
