src/checker.v
@@ -4,42 +4,86 @@ Require Import ch2o.prelude.base.
 Require Import Coq.Strings.String.
 Require Import Coq.Bool.Sumbool.
 Require Import common.
+Open Scope string_scope.
 
 Definition ty_ctx := stringmap ty.
 
-Section checker.
-Context (P: program).
-Context (Γ: ty_ctx).
+Class Viewpoint (A B C: Type) := adapt_viewpoint: A -> B -> option C.
+Notation "a ▷ b" := (adapt_viewpoint a b) (at level 60, right associativity) : C_scope.
 
-Class Viewpoint (A B: Type) := adapt_viewpoint: A -> B -> B.
-Notation "a ⊳ b" := (adapt_viewpoint a b) (at level 60, right associativity) : C_scope.
+Class ExtractViewpoint (A B C: Type) := extract_viewpoint: A -> B -> option C.
+Notation "a ▶ b" := (extract_viewpoint a b) (at level 60, right associativity) : C_scope.
 
 Class Alias (A: Type) := alias: A -> A.
+Class Unalias (A: Type) := unalias: A -> A.
+
 Class Subtype (A: Type) := is_subtype: A -> A -> bool.
 
-Instance viewpoint_cap: Viewpoint cap cap := {
+Instance viewpoint_cap: Viewpoint ecap cap cap := {
   adapt_viewpoint a b := match a, b with
-  | cap_iso, cap_iso => cap_iso
-  | cap_iso, cap_ref => cap_iso
+  | cap_iso_eph, cap_iso => Some cap_iso
+  | cap_iso_eph, cap_ref => Some cap_iso
 
-  | cap_ref, cap_iso => cap_iso
-  | cap_ref, cap_ref => cap_ref
+  | cap_iso, cap_iso => Some cap_iso
+  | cap_iso, cap_ref => Some cap_iso
 
-  | _, cap_tag => cap_tag
+  | cap_ref, cap_iso => Some cap_iso
+  | cap_ref, cap_ref => Some cap_ref
 
-  | cap_tag, _ => cap_tag
+  | cap_tag, _ => None
+  | _, cap_tag => Some cap_tag
   end
 }.
 
-Instance viewpoint_cap_ty: Viewpoint cap ty := {
+Instance extract_viewpoint_cap: ExtractViewpoint ecap cap ecap := {
+  extract_viewpoint a b := match a, b with
+  | cap_iso_eph, cap_iso => Some cap_iso_eph
+  | cap_iso_eph, cap_ref => Some cap_iso_eph
+  | cap_iso_eph, cap_tag => Some (ecap_cap cap_tag)
+
+  | cap_iso, cap_iso => Some cap_iso_eph
+  | cap_iso, cap_ref => Some (ecap_cap cap_tag)
+  | cap_iso, cap_tag => Some (ecap_cap cap_tag)
+
+  | cap_ref, cap_iso => Some cap_iso_eph
+  | cap_ref, cap_ref => Some (ecap_cap cap_ref)
+  | cap_ref, cap_tag => Some (ecap_cap cap_tag)
+
+  | cap_tag, _ => None
+  end
+}.
+
+Instance viewpoint_cap_ty: Viewpoint ecap ty ty := {
   adapt_viewpoint a b := match b with
-  | ty_name n c => ty_name n (a ⊳ c)
+  | ty_name n (ecap_cap c) =>
+      c' <- a ▷ c;
+      Some (ty_name n (ecap_cap c'))
+  | ty_name n (ecap_iso_eph) => None
   end
 }.
 
-Instance alias_cap : Alias cap := {
+Instance extract_viewpoint_cap_ty: ExtractViewpoint ecap ty ty := {
+  extract_viewpoint a b := match b with
+  | ty_name n (ecap_cap c) =>
+      c' <- a ▶ c;
+      Some (ty_name n c')
+  | ty_name n (ecap_iso_eph) => None
+  end
+}.
+
+Instance alias_cap : Alias ecap := {
   alias a := match a with
+  | cap_iso_eph => cap_iso
   | cap_iso => cap_tag
+  | cap_ref => cap_ref
+  | cap_tag => cap_tag
+  end
+}.
+
+Instance unalias_cap : Unalias ecap := {
+  unalias a := match a with
+  | cap_iso_eph => cap_iso
+  | cap_iso => cap_iso_eph
   | cap_ref => cap_ref
   | cap_tag => cap_tag
   end
@@ -51,57 +95,92 @@ Instance alias_ty : Alias ty := {
   end
 }.
 
-Instance subtype_cap : Subtype cap := {
-  is_subtype a b := match a, b with
-  | cap_iso, cap_iso => true
-  | _, cap_tag => true
-  | _, _ => false
+Instance unalias_ty : Unalias ty := {
+  unalias a := match a with
+  | ty_name n c => ty_name n (unalias c)
   end
 }.
 
-Instance subtype_ty : Subtype ty := {
+Instance subtype_cap : Subtype ecap := {
   is_subtype a b :=
+    trace (a, b) $
     match a, b with
-    | ty_name name_a cap_a, ty_name name_b cap_b =>
-        if string_dec name_a name_b
-        then is_subtype cap_a cap_b
+    | cap_iso_eph, _ => true
+    | cap_iso, cap_iso => true
+    | cap_ref, cap_ref => true
+    | _, cap_tag => true
+    | _, _ => false
+    end
+}.
+
+Definition string_beq a b := if string_dec a b then true else false.
+
+Instance subtype_ty : Subtype ty := {
+  is_subtype sub super :=
+    trace (sub, super) $
+    match sub, super with
+    | ty_name name_sub cap_sub, ty_name name_super cap_super =>
+        if string_beq name_sub name_super || string_beq name_super "Any" || string_beq name_sub "Null"
+        then is_subtype cap_sub cap_super
         else false
     end
 }.
 
-Fixpoint ck_expr (e: expr) : option ty :=
+Section checker.
+Context (P: program).
+
+Fixpoint ck_expr (Γ: ty_ctx) (e: expr) : option ty :=
+  let ck_alias (e: expr) (expected: ty) : option unit :=
+    ety <- ck_expr Γ e;
+    if is_subtype ety (unalias expected)
+    then Some ()
+    else None in
+
   match e with
+  | expr_null => Some (ty_name "Null" cap_iso_eph)
+
+  | expr_seq e1 e2 =>
+      ty1 <- ck_expr Γ e1;
+      ty2 <- ck_expr Γ e2;
+      Some ty2
+
   | expr_local x => Γ !! x
-  | expr_field e f =>
-      baset <- ck_expr e;
-      match baset with
-      | ty_name name cap =>
-          cls <- lookup_class name P;
-          fty <- lookup_field f cls;
-          Some (cap ⊳ fty)
-      end
 
   | expr_assign_local x e =>
-      lhs <- Γ !! x;
-      rhs <- ck_expr e;
-      if is_subtype (alias rhs) lhs
-      then Some lhs
-      else None
+      lhs_ty <- Γ !! x;
+      _ <- ck_alias e lhs_ty;
+      Some (unalias lhs_ty)
 
-  | expr_ctor name ctor_name es =>
-      cls <- lookup_class name P;
-      '(args, _) <- lookup_ctor ctor_name cls;
-      _ <- ck_args es (map snd args);
+  | expr_field e f =>
+      base_ty <- ck_expr Γ e;
+      match base_ty with
+      | ty_name ds cap =>
+          field_ty <- lookup_F P ds f;
+          cap ▷ field_ty
+      end
 
-      Some (ty_name name cap_ref)
+  | expr_assign_field e f e' =>
+      base_ty <- ck_expr Γ e;
+      match base_ty with
+      | ty_name ds cap =>
+          field_ty <- lookup_F P ds f;
+          _ <- ck_alias e' field_ty;
+          (*cap ▶ field_ty*)
+          Some field_ty
+      end
+
+  | expr_ctor kt k es =>
+      '(_, args, _) <- lookup_Md P kt k;
+      _ <- ck_args Γ es (map snd args);
+
+      Some (ty_name kt cap_ref)
 
   | expr_call e0 m es =>
-      baset <- ck_expr e0;
+      baset <- ck_expr Γ e0;
       match baset with
-      | ty_name name cap =>
-          cls <- lookup_class name P;
-          '(reccap, args, retty, _) <- lookup_method m cls;
-          _ <- ck_args es (map snd args);
+      | ty_name ds cap =>
+          '(_, args, retty) <- lookup_Md P ds m;
+          _ <- ck_args Γ es (map snd args);
 
           Some retty
       end
@@ -109,14 +188,51 @@ Fixpoint ck_expr (e: expr) : option ty :=
   | _ => None
   end
 with
-  ck_args (es: list_expr) (args: list ty) : option unit :=
+  ck_args (Γ: ty_ctx) (es: list_expr) (args: list ty) : option unit :=
+    let ck_alias (e: expr) (expected: ty) : option unit :=
+      ety <- ck_expr Γ e;
+      if is_subtype ety (unalias expected)
+      then Some ()
+      else None in
+
     match es, args with
     | list_expr_nil, nil => Some ()
     | list_expr_cons e es', arg :: args' =>
-        ety <- ck_expr e;
-        if is_subtype (alias ety) arg
-        then ck_args es' args'
-        else None
+        _ <- ck_alias e arg;
+        ck_args Γ es' args'
     | _, _ => None
-    end.
+    end
+.
+
+Definition wf_method (name: string) (receiver: ty) (args_ty: list (string * ty)) (ret_ty: ty) (body: expr) : option unit :=
+  let Γ : ty_ctx := map_of_list (("this", receiver)::args_ty) in
+  body_ty <- ck_expr Γ body;
+  if is_subtype body_ty ret_ty
+  then Some ()
+  else None.
+
+Definition wf_ctor (ds: string) (kt: ctor) : option unit :=
+  let '(k, (args_ty, body)) := kt in
+  let receiver := ty_name ds cap_ref in
+  wf_method k receiver args_ty receiver body.
+
+Definition wf_func (ds: string) (mt: func) : option unit :=
+  let '(m, (recv_cap, args_ty, ret_ty, body)) := mt in
+  let receiver := ty_name ds recv_cap in
+  wf_method m receiver args_ty ret_ty body.
+
+Definition wf_class (ct : class) : option unit :=
+  let '(ds, (fs, ks, ms)) := ct in
+  _ <- mapM (wf_ctor ds) ks;
+  _ <- mapM (wf_func ds) ms;
+  Some ().
+
+Definition wf_actor (cl : actor) : option unit := None.
+
+Definition wf_program : option unit :=
+  let '(nts, sts, cts, ats) := P in
+  _ <- mapM wf_class cts;
+  _ <- mapM wf_actor ats;
+  Some ().
+
 End checker.
