src/common.v
@@ -1,5 +1,6 @@
 Require Import ch2o.prelude.nmap.
 Require Import ch2o.prelude.base.
+Require Import Coq.Strings.String.
 
 Notation "m >>= f" := (mbind f m) (at level 60, right associativity) : C_scope.
 Notation "( m >>=)" := (λ f, mbind f m) (only parsing) : C_scope.
@@ -24,3 +25,50 @@ Notation "' ( x1 , x2 , x3  , x4 , x5 ) <- y ; z" :=
 Notation "' ( x1 , x2 , x3  , x4 , x5 , x6 ) <- y ; z" :=
   (y >>= (λ x : _, let ' (x1,x2,x3,x4,x5,x6) := x in z))
   (at level 65, only parsing, right associativity) : C_scope.
+
+Class Zip (A: Type) (B: Type) (C: Type) := zip: list A -> B -> list (A*C).
+
+Instance zip_list {A} {B} : Zip A (list B) B :=
+  let fix z a b := match a, b with
+  | ah::a', bh::b' => (ah, bh)::(z a' b')
+  | nil, _ => nil
+  | _, nil => nil
+  end in z.
+
+Instance zip_one {A} {B} : Zip A B B :=
+  let fix z a b := match a with
+  | ah::a' => (ah, b)::(z a' b)
+  | nil => nil
+  end in z.
+
+Fixpoint insert_all {K: Type} {A: Type} {M: Type} {i: Insert K A M} (l: list (K*A)) (m: M) : M :=
+  match l with
+  | (k,a)::l' => insert_all l' (insert k a m)
+  | nil => m
+  end.
+
+Definition insertZip {A: Type} {B: Type} {C: Type} {M: Type} {i: Insert A C M} {z: Zip A B C} (a: list A) (b: B)
+  := insert_all (zip a b).
+
+Notation "<[* k := a ]>" := (insertZip k a)
+  (at level 5, right associativity, format "<[* k := a ]>") : C_scope.
+
+Instance list_tuple_lookup {B} : Lookup string B (list (string * B)) := {
+  lookup :=
+    let fix look k l := match l with
+    | (k', v)::tail => 
+        if string_dec k k'
+        then Some v
+        else look k tail
+    | nil => None
+    end in look
+}.
+
+Fixpoint mapM {A B: Type} {M: Type -> Type} {r: MRet M} {b: MBind M} (f: A -> M B) (xs: list A) : M (list B) :=
+  match xs with
+  | x::tail => f x >>= (λ y, mapM f tail >>= (λ ys, mret (y :: ys)))
+  | nil => mret nil
+  end.
+
+Definition trace {A B: Type} (_: A) (x: B) := x.
+Definition traceId {A: Type} (x: A) := x.
